Tactic/signature.lean
@@ -1,0 +1,74 @@
+import Lean
+import Mathlib.Data.Quot
+
+open Lean Elab Tactic Term Meta
+
+/-
+From:
+  https://github.com/FWuermse/grw/blob/main/Grw/Morphism.lean
+{
+-/
+def relation (α : Sort u) := α → α → Prop
+
+def respectful {α : Sort u} {β : Sort v} (r : relation α) (r' : relation β) : relation (α → β) :=
+  fun f g => ∀ x y, r x y → r' (f x) (g y)
+notation:55 r " ⟹ " r' => respectful r r'
+
+def Signature {α : Sort u} (m : α) (r : relation α) := r m m
+/-
+                                        }
+-/
+
+/-
+We will be considering respectful operations of the form:
+  f_sig : α₁ → ⋯ → αₘ → Signature f (R₁ ⟹ R₂)
+  f_sig : α₁ → ⋯ → αₘ → Signature f (R₁ ⟹ R₂ ⟹ R₃)
+  f_sig : α₁ → ⋯ → αₘ → Signature f (R₁ ⟹ Eq)
+  f_sig : α₁ → ⋯ → αₘ → Signature f (R₁ ⟹ R₂ ⟹ Eq)
+-/
+
+
+--Does NOT Typecheck #check fun n => Quotient.map₂_mk (Nat.add) (add_sig n)
+
+def arrowsToLift (arrows : Expr) : Option Name :=
+  match arrows with
+    | .app (.app (.app (.app (.const ``respectful _) _) _) R₁) arrows  =>
+      match arrows with
+                                    --Signature f (R₁ ⟹ Eq)
+      | .app (.const ``Eq _) _  => return ``Quotient.lift_mk
+                                                  --Signature f (R₁ ⟹ R₂)
+      | .app (.app (.const ``Setoid.r _) _) _    => return ``Quotient.map_mk
+      | .app R₂ arrows =>
+        match arrows with
+                                      --Signature f (R₁ ⟹ R₂ ⟹ Eq)
+        | .app (.const ``Eq _) _ => return ``Quotient.lift₂_mk
+                                      --Signature f (R₁ ⟹ R₂ ⟹ R₃)
+        | .app (.app (.const ``Setoid.r _) _) _ => return ``Quotient.map₂_mk
+
+        | _ => none
+      | _ => none
+    | _ => none
+
+
+def letSignature (f : Name) (f_sig : Expr) : TacticM Unit := do
+  let f_sigType := ← inferType f_sig
+
+  -- eq_pf := fun α₁ ... αₙ => liftFxn (f₁) (f_sig α₁ ... αₙ)
+  let eq_pf   := ← forallTelescope f_sigType fun alphas sig_f₁_arrows₁ => do
+    let f₁                   := (sig_f₁_arrows₁.getAppArgs)[1]!
+    let arrows₁              := (sig_f₁_arrows₁.getAppArgs)[2]!
+    let .some liftFxn       := arrowsToLift arrows₁ | throwError "Must have type ∀ α₁ ... αₙ, Signature f₁ (R₁ ⟹ ...)"
+    mkLambdaFVars alphas (← mkAppM liftFxn #[f₁, (← mkAppM' f_sig alphas)])
+  let eq_Type := ← inferType eq_pf
+
+  withMainContext do
+    liftMetaTactic fun mvarId => do
+      let mvarIdNew ← mvarId.define (f.appendAfter "_eq") eq_Type eq_pf
+      let (_, mvarIdNew) ← mvarIdNew.intro1P
+      return [mvarIdNew]
+
+elab "letSignature" f:ident f_sig:term : tactic =>
+  do
+  let f := f.getId
+  let f_sig := ← Tactic.elabTerm f_sig none
+  letSignature (f) (f_sig)
